label-free/Substitution.v
@@ -13,67 +13,60 @@ end.
 
 (* Term substitution *)
 
-(* We want to substitute M for nth hyp. in term N0, provided that the current context
-   is ctx. *)
-Fixpoint subst_t_outer (M0: te_LF) (n: nat) (ctx: ctx_LF) (N0: te_LF) (curr: ctx_LF) {struct N0} :=
+(* We want to substitute M for nth hyp. in term N0, provided that the current context is ctx. *)
+Fixpoint subst_t_outer (M0: te_LF) (n: nat) (ctx: ctx_LF) (N0: te_LF) {struct N0} :=
 match N0 with
 | hyp_LF n => 
     hyp_LF n
 | lam_LF A M => 
-    lam_LF A (subst_t_outer M0 n ctx M curr)
+    lam_LF A (subst_t_outer M0 n ctx M)
 | appl_LF M N => 
-    appl_LF (subst_t_outer M0 n ctx M curr) (subst_t_outer M0 n ctx N curr)
+    appl_LF (subst_t_outer M0 n ctx M) (subst_t_outer M0 n ctx N)
 | box_LF M => 
-  let w0 := var_gen (free_worlds_LF N0) in (* shouldn't we add sth? *)
-    box_LF (subst_t_outer M0 n ctx M (fctx w0))
+    box_LF (subst_t_outer M0 n ctx M)
 | unbox_fetch_LF w M => 
-  match (eq_ctx_LF_dec ctx w) with
-    | left _ => unbox_fetch_LF w (subst_t_inner M0 n M ctx) 
-    | right _ => unbox_fetch_LF w (subst_t_outer M0 n ctx M w)
-  end
+  let M' := If (ctx = w) then subst_t_inner M0 n M ctx
+            else subst_t_outer M0 n ctx M in
+    unbox_fetch_LF w M'
 | get_here_LF w M =>
-  match (eq_ctx_LF_dec ctx w) with
-    | left _ => get_here_LF w (subst_t_inner M0 n M ctx) 
-    | right _ => get_here_LF w (subst_t_outer M0 n ctx M w)
-  end
+  let M' := If (ctx = w) then subst_t_inner M0 n M ctx
+            else subst_t_outer M0 n ctx M in
+    get_here_LF w M'        
 | letdia_get_LF w M N =>
-  match (eq_ctx_LF_dec ctx w) with
-    | left _ => letdia_get_LF w (subst_t_inner M0 n M ctx) (subst_t_outer M0 n ctx N w)
-    | right _ => letdia_get_LF w (subst_t_outer M0 n ctx M w) (subst_t_outer M0 n ctx N w)
-  end
+  let M' := If (ctx = w) then subst_t_inner M0 n M ctx
+            else subst_t_outer M0 n ctx M in
+  let N' := subst_t_outer M0 n ctx N in
+    letdia_get_LF w M' N'
 end
 (* Current context is exactly the context in which we want to do susbtitution *)
-with subst_t_inner (M0: te_LF) (m: nat) (N0: te_LF) (curr: ctx_LF) {struct N0} :=
+with subst_t_inner (M0: te_LF) (n: nat) (N0: te_LF) (curr: ctx_LF) {struct N0} :=
 match N0 with
-| hyp_LF n => 
-    if (eq_nat_dec n m) then M0 else hyp_LF n
+| hyp_LF m => 
+    if (eq_nat_dec m n) then M0 else hyp_LF m
 | lam_LF A M => 
-    lam_LF A (subst_t_inner M0 (S m) M curr)
+    lam_LF A (subst_t_inner M0 (S n) M curr)
 | appl_LF M N => 
-    appl_LF (subst_t_inner M0 m M curr) (subst_t_inner M0 m N curr)
+    appl_LF (subst_t_inner M0 n M curr) (subst_t_inner M0 n N curr)
 | box_LF M =>
-  let w0 := var_gen (free_worlds_LF N0) in
-    box_LF (subst_t_outer M0 m curr M (fctx w0))
+    box_LF (subst_t_outer M0 n curr M)
 | unbox_fetch_LF w M =>
-  match (eq_ctx_LF_dec curr w) with
-    | left _ => unbox_fetch_LF w (subst_t_inner M0 m M curr) 
-    | right _ => unbox_fetch_LF w (subst_t_outer M0 m curr M w)
-  end
+  let M' := If (curr = w) then subst_t_inner M0 n M curr
+            else subst_t_outer M0 n curr M in
+    unbox_fetch_LF w M'
 | get_here_LF w M =>
-  match (eq_ctx_LF_dec curr w) with
-    | left _ => get_here_LF w (subst_t_inner M0 m M curr) 
-    | right _ => get_here_LF w (subst_t_outer M0 m curr M w)
-  end
+  let M' := If (curr = w) then subst_t_inner M0 n M curr
+            else subst_t_outer M0 n curr M in
+    get_here_LF w M'
 | letdia_get_LF w M N =>
-  match (eq_ctx_LF_dec curr w) with
-    | left _ => letdia_get_LF w (subst_t_inner M0 m M curr) (subst_t_outer M0 m curr N w)
-    | right _ => letdia_get_LF w (subst_t_outer M0 m curr M w) (subst_t_outer M0 m curr N w)
-  end
+  let M' := If (curr = w) then subst_t_inner M0 n M curr
+            else subst_t_outer M0 n curr M in
+  let N' := subst_t_inner M0 n N curr in
+    letdia_get_LF w M' N'
 end.
 
 Definition subst_t M n ctx N curr :=
   If ctx = curr then (subst_t_inner M n N curr) 
-  else (subst_t_outer M n ctx N curr). 
+  else (subst_t_outer M n ctx N). 
 
 Notation " [ M // n | ctx ] [ N | curr ] " := 
   (subst_t M n ctx N curr) (at level 5) : label_free_is5_scope.
@@ -110,10 +103,10 @@ match M0 with
 | appl_LF M N => appl_LF (subst_ctx_outer M curr ctx1 ctx2 len_old) 
                          (subst_ctx_outer N curr ctx1 ctx2 len_old)
 | box_LF M => 
-  let w0 := var_gen (free_worlds_LF M) in
+  let w0 := var_gen (free_worlds_LF M \u (var_from ctx1) \u 
+                     (var_from ctx2) \u (var_from curr)) in
   let (ctx1', ctx2') := recalculate_ctx ctx1 ctx2 in 
     box_LF (subst_ctx_outer M (fctx w0) ctx1' ctx2' len_old)
-
 
 | unbox_fetch_LF w M => 
   match (eq_ctx_LF_dec w ctx1) with
@@ -219,8 +212,8 @@ match M0 with
     box_LF (subst_ctx_outer M (fctx w0) ctx1' ctx2' len_old)
 
 | unbox_fetch_LF w M =>
-  match (eq_ctx_LF_dec w ctx2) with
-    | left _ => unbox_fetch_LF w (subst_ctx_old M ctx1 ctx2 len_old)
+  match (eq_ctx_LF_dec w ctx1) with
+    | left _ => unbox_fetch_LF w (subst_ctx_new M ctx1 ctx2 len_old)
     | right _ => 
       match (eq_ctx_LF_dec w ctx2) with 
         | left _ => unbox_fetch_LF ctx1 (subst_ctx_old M ctx1 ctx2 len_old)
@@ -254,18 +247,15 @@ match M0 with
 end.
 
 Definition subst_ctx M c1 c2 curr len_old :=
-match (eq_ctx_LF_dec c1 c2) with
-| left _ => M
-| right _ => 
-  match (eq_ctx_LF_dec curr c1) with
-  | left _ => subst_ctx_new M c1 c2 len_old
-  | right _ => 
-    match (eq_ctx_LF_dec curr c2) with
-    | left _ => subst_ctx_old M c1 c2 len_old
-    | right _ => subst_ctx_outer M curr c1 c2 len_old
-    end
-  end
-end.
+If c1 = c2 then M
+else
+  If curr = c1 then
+    subst_ctx_new M c1 c2 len_old
+  else
+    If curr = c2 then
+      subst_ctx_old M c1 c2 len_old
+    else
+      subst_ctx_outer M curr c1 c2 len_old.
 
 Notation " {{ c1 // c2 }} [ M | curr , m ] " := 
   (subst_ctx M c1 c2 curr m) (at level 5) : label_free_is5_scope.
@@ -289,7 +279,7 @@ Qed.
 Lemma subst_t__outer:
 forall M k N w w'
   (Neq: w <> w'),
-  subst_t_outer M k w N w' = [M//k | w] [N | w'].
+  subst_t_outer M k w N = [M//k | w] [N | w'].
 intros; unfold subst_t;
 case_if; reflexivity.
 Qed.
@@ -324,6 +314,130 @@ intros;
 unfold subst_ctx;
 repeat case_if;
 reflexivity.
+Qed.
+
+Lemma generate_fresh:
+forall M w
+  (HIn: w \in M),
+  var_gen M <> w.
+Admitted.
+
+Lemma no_unbound_worlds_LF_subst_w_id:
+forall M n
+  (H_unbound: unbound_worlds n M = nil),
+  forall w w0, {{ w // bctx n }} [M | w0, 0] = M.
+induction M; intros; unfold subst_ctx.
+(* hyp *)
+repeat case_if; reflexivity.
+(* lam *)
+unfold subst_ctx in *;
+simpl in H_unbound.
+specialize IHM with n w w0.
+apply IHM with (w:=w) (w0:=w0) in H_unbound.
+repeat case_if; simpl; 
+try rewrite H_unbound; 
+auto.
+(* appl *)
+unfold subst_ctx in *;
+simpl in H_unbound;
+apply app_eq_nil in H_unbound;
+destruct H_unbound as (H_Un1, H_Un2);
+apply IHM1 with (w:=w) (w0:=w0) in H_Un1;
+apply IHM2 with (w:=w) (w0:=w0) in H_Un2;
+repeat case_if; simpl;
+try (rewrite H_Un1; rewrite H_Un2); reflexivity.
+(* box *)
+inversion H_unbound; subst.
+apply IHM with (w:=w) (w0:=w0) in H0. 
+repeat case_if; simpl; try subst; auto.
+destruct w.
+rewrite subst_ctx__outer;
+unfold recalc_simpl_ctx; try discriminate;
+assert ({{bctx (S n0) // bctx (S n)}}[M
+     | fctx (var_gen (free_worlds_LF M \u var_from (bctx n0) \u \{})), 0] = M) by
+  (eapply IHM with (n:=S n); simpl in H_unbound; assumption).
+rewrite H2; reflexivity.
+intro nn; inversion nn; subst n0; elim H; reflexivity.
+subst w0;
+rewrite subst_ctx__outer;
+unfold recalc_simpl_ctx; try discriminate.
+rewrite IHM; eauto.
+assert (v \in free_worlds_LF M \u var_from (fctx v) \u \{}).
+repeat rewrite in_union; right; left; simpl; rewrite in_singleton; reflexivity.
+intro. inversion H2. symmetry in H4.
+eapply generate_fresh; eauto. 
+subst w0; destruct w.
+rewrite subst_ctx__outer;
+unfold recalc_simpl_ctx; try discriminate.
+assert ({{bctx (S n0) // bctx (S n)}}[M
+     | fctx (var_gen (free_worlds_LF M \u var_from (bctx n0) \u \{})), 0] = M) by
+  (eapply IHM with (n:=S n); simpl in H_unbound; assumption).
+rewrite H2; reflexivity.
+intro nn; inversion nn; subst n0; elim H; reflexivity.
+rewrite subst_ctx__outer;
+unfold recalc_simpl_ctx; try discriminate.
+rewrite IHM; eauto.
+assert (v \in free_worlds_LF M \u var_from (fctx v) \u \{}).
+repeat rewrite in_union; right; left; simpl; rewrite in_singleton; reflexivity.
+intro. inversion H3. symmetry in H5.
+eapply generate_fresh; eauto. 
+destruct w.
+rewrite subst_ctx__outer;
+unfold recalc_simpl_ctx; try discriminate.
+rewrite IHM; eauto.
+intro nn; inversion nn; subst n0; elim H; reflexivity.
+rewrite subst_ctx__outer;
+unfold recalc_simpl_ctx; try discriminate.
+rewrite IHM; eauto.
+assert (v \in free_worlds_LF M \u var_from (fctx v) \u \{} \u var_from w0).
+repeat rewrite in_union; right; left; simpl; rewrite in_singleton; reflexivity.
+intro. inversion H4. symmetry in H6.
+eapply generate_fresh; eauto. 
+(* unbox_fetch *)
+inversion H_unbound; destruct c; simpl; try discriminate.
+repeat case_if; simpl;
+try rewrite subst_ctx__old;
+try rewrite subst_ctx__new;
+try rewrite subst_ctx__outer;
+try discriminate;
+try rewrite IHM; 
+eauto.
+subst w; reflexivity.
+(* get_here *)
+inversion H_unbound; destruct c; simpl; try discriminate.
+repeat case_if; simpl;
+try rewrite subst_ctx__old;
+try rewrite subst_ctx__new;
+try rewrite subst_ctx__outer;
+try discriminate;
+try rewrite IHM; 
+eauto.
+(* letdia_get *)
+inversion H_unbound; destruct c; simpl; try discriminate.
+apply app_eq_nil in H0; destruct H0.
+repeat case_if; simpl;
+unfold recalc_simpl_ctx in *; 
+destruct w; destruct w0;
+try repeat rewrite subst_ctx__old;
+try repeat rewrite subst_ctx__new;
+try repeat rewrite subst_ctx__outer;
+try discriminate;
+try rewrite IHM1;
+try rewrite IHM2; 
+eauto;
+try (intro nn; inversion nn; subst; elim H1; reflexivity);
+try (intro nn; inversion nn; subst; elim H3; reflexivity).
+intro nn; inversion nn; subst; elim H2; reflexivity.
+Qed.
+
+Lemma closed_ctx_subst_id:
+forall M w n curr
+  (H_lc: lc_w_n_LF M n),
+  {{w // bctx n}} [ M | curr, 0] = M.
+intros;
+apply no_unbound_worlds_LF_subst_w_id;
+apply closed_no_unbound_worlds;
+assumption.
 Qed.
 
 End Lemmas.
